Move projectS to choreoUtils

utils/choreoUtilsScript.sml
@@ -216,4 +216,79 @@ Proof
   rw[nub'_def,nub'_FILTER,FILTER_FILTER]
 QED
 
+(* Project a global state `(proc,var) |-> val` into a single process
+   state `var |-> val`
+*)
+Definition projectS_def:
+  projectS p s = MAP_KEYS (λx. FST x) (DRESTRICT s (λx. SND x = p))
+End
+
+(* The domain of a state `s` projected to a process `p` is the set of
+   all variable names associated with `p` in the domain of `s`
+*)
+Theorem fdom_projectS:
+  ∀p s. FDOM (projectS p s) = { v | (v,p) ∈ FDOM s }
+Proof
+  rw [projectS_def,MAP_KEYS_def,DRESTRICT_DEF,IMAGE_DEF,FUN_EQ_THM]
+  \\ EQ_TAC >> rw [] >> fs [] >> Q.EXISTS_TAC `(x,p)` >> rw []
+QED
+
+
+(* If a key `(v,p)` is in the domain of a global state `s` then
+   one can expect the application of the projected key `v` over
+   a projected state `projectS p s` to be equal to an original
+   (un-projected) application
+*)
+Theorem fapply_projectS:
+  ∀p v (s : β # α |-> γ). (v,p) ∈ FDOM s ⇒ projectS p s ' v = s ' (v,p)
+Proof
+  rw [projectS_def,MAP_KEYS_def,DRESTRICT_DEF]
+  \\ sg `INJ FST (FDOM (DRESTRICT s (λx. SND x = p))) 𝕌(:β)`
+  >- rw [DRESTRICT_DEF,INJ_DEF,PAIR_FST_SND_EQ]
+  \\ IMP_RES_TAC (MAP_KEYS_def |> CONV_RULE (TOP_DEPTH_CONV FORALL_AND_CONV) |> CONJUNCT2)
+  \\ first_x_assum (ASSUME_TAC o Q.SPEC `(v,p)`)
+  \\ rfs [DRESTRICT_DEF,ETA_THM]
+QED
+
+(* If a value is available on a state `s` with key `(v,p)` then it
+   should also be available in a projected state `projectS p s` with
+   key `v`
+*)
+Theorem lookup_projectS:
+  ∀p v s d. FLOOKUP s (v,p) = SOME d ⇒ FLOOKUP (projectS p s) v = SOME d
+Proof
+  rw [FLOOKUP_DEF,fapply_projectS,fdom_projectS]
+QED
+
+(* Alternative version of lookup_projectS *)
+Theorem lookup_projectS':
+  ∀p v s d. FLOOKUP s (v,p) = FLOOKUP (projectS p s) v
+Proof
+  rw [FLOOKUP_DEF,fapply_projectS,fdom_projectS]
+QED
+
+(* If a state is updated with bindings for a process (`p2`) this does not
+   affect the projection of any other process (`p1`)
+*)
+Theorem fupdate_projectS:
+  ∀p1 p2 s v d. p1 ≠ p2 ⇒ projectS p1 (s |+ ((v,p2),d)) = projectS p1 s
+Proof
+  rw [projectS_def]
+QED
+
+(*  Updating a projected state is equivalent to updating
+    a global state with the corresponding process
+
+*)
+Theorem projectS_fupdate:
+  ∀p v d s. projectS p (s |+ ((v,p),d)) = projectS p s |+ (v,d)
+Proof
+  rw [projectS_def]
+  \\ sg `INJ FST ((v,p) INSERT FDOM (DRESTRICT s (λx. SND x = p))) 𝕌(:β)`
+  >- REPEAT (rw [DRESTRICT_DEF,INJ_DEF,PAIR_FST_SND_EQ])
+  \\ IMP_RES_TAC (MAP_KEYS_FUPDATE)
+  \\ first_x_assum (ASSUME_TAC o Q.SPEC `d`)
+  \\ rfs [DRESTRICT_DEF,ETA_THM]
+QED
+
 val _ = export_theory ()
